removed PrettyBounds from TM

theories/L/Datatypes/LBool.v
@@ -11,7 +11,34 @@ MetaCoq Run (tmGenEncodeInj "bool_enc" bool).
 (* For each encoding, Lrewrite must contain an lemma that solves goals like "encode b s t >* match ...end". The database Lrewrite also calls Lproc to discharge the other assumptions *)
 #[export] Hint Resolve bool_enc_correct : Lrewrite.
 
-(* register thefunctional constructors (not neccessary here) *)
+(* register the functional constructors (not neccessary here) *)
+
+Class eqbClass X (eqb : X -> X -> bool): Type := 
+  _eqb_spec : forall (x y:X), reflect (x=y) (eqb x y).
+
+#[export] Hint Mode eqbClass + -: typeclass_instances. (* treat argument as input and force evar-freeness*)
+
+Definition eqb X eqb `{H:eqbClass (X:=X) eqb} := eqb.
+
+Arguments eqb {_ _ _}: simpl never.
+
+Lemma eqb_spec {X} {f : X -> X -> bool} {_:eqbClass f}:
+  forall (x y:X), reflect (x=y) (eqb x y).
+Proof.
+  intros. eapply _eqb_spec.
+Qed.
+
+#[global]
+Instance eqbBool_inst : eqbClass Bool.eqb.
+Proof.
+  intros ? ?. eapply iff_reflect. rewrite eqb_true_iff. reflexivity.
+Qed.
+
+#[global]
+Instance term_eqb_bool : computable Bool.eqb.
+Proof.
+  extract.
+Qed.
 
 #[global]
 Instance term_negb : computable negb.
