theories/L/Reductions/H10_to_L.v
@@ -3,7 +3,7 @@ Require Import Undecidability.PCP.Util.PCP_facts.
 Require Import Undecidability.Shared.Libs.PSL.FiniteTypes Undecidability.Shared.Libs.PSL.FiniteTypes.Arbitrary.
 From Undecidability.Synthetic Require Export DecidabilityFacts EnumerabilityFacts ListEnumerabilityFacts ReducibilityFacts.
 From Undecidability.L.Datatypes Require Import LNat LProd.
-From Undecidability.L.Datatypes.List Require Import List_basics List_eqb List_fold List_enc.
+From Undecidability.L.Datatypes.List Require Import List_basics List_eqb List_enc.
 
 From Undecidability.L Require Import Tactics.LTactics Computability.MuRec Computability.Synthetic Tactics.GenEncode.
 From Undecidability.Shared.Libs.DLW.Vec Require Import pos.
