theories/L/Reductions/MuRec/MuRec_extract.v
@@ -1,5 +1,5 @@
 From Undecidability.L.Datatypes Require Import LNat LOptions LSum.
-From Undecidability.L.Datatypes.List Require Import List_basics List_eqb List_fold List_enc.
+From Undecidability.L.Datatypes.List Require Import List_basics List_eqb List_enc.
 
 Require Import Undecidability.L.Tactics.GenEncode.
 
