theories/L/Tactics/mixedTactics.v
@@ -14,15 +14,5 @@ Tactic Notation "destruct" "_" "eqn" ":" ident(E)   :=
 Tactic Notation "destruct" "*" :=
   repeat destruct _.
 
-Ltac dec :=
-  match goal with
-    | [ |- context[Dec ?X] ] => decide X
-  end.
-
-Ltac trace :=
-  match goal with
-    |- ?G => idtac "Trace:";idtac G
-  end.
-
 Tactic Notation (at level 3) "repeat'" tactic3(t) :=
   let rec loop := (once t);try loop in loop.
