theories/TM/Single/EncodeTapes.v
@@ -4,10 +4,7 @@ Require Export Undecidability.TM.Basic.Mono Undecidability.TM.Compound.Multi.
 (* the above imports sidestep the import of ProgrammingTools below to avoid the dependency on Hoare *)
 (*From Undecidability.TM Require Import ProgrammingTools.*)
 
-From Undecidability.TM.PrettyBounds Require Export SizeBounds.
-
 From Undecidability Require Import TM.Util.VectorPrelim.
-
 
 Inductive sigTape (sig : Type) : Type :=
 | LeftBlank (marked : bool)
@@ -36,7 +33,6 @@ Proof.
   - rewrite <- countSplit. rewrite countMap_injective, countMap_zero by congruence. now rewrite enum_ok.
   - rewrite <- countSplit. rewrite countMap_injective, countMap_zero by congruence. now rewrite enum_ok.
 Qed.
-
 
 Definition isMarked (sig : Type) (s : sigTape sig) : bool :=
   match s with
@@ -91,20 +87,6 @@ Instance Encode_tape (sig : Type) : codable (sigTape sig) (tape sig) :=
 (* Compute encode_tape (leftof 1 [2;3]). *)
 (* Compute encode_tape (rightof 3 [2;1]). *)
 
-
-(* Moving does not change the number of symbols. *)
-Goal forall (sig : Type) (m : move) (t : tape sig), length (encode_tape (tape_move t m)) = length (encode_tape t).
-Proof.
-  intros.
-  destruct m eqn:E1, t eqn:E2; cbn; auto.
-  - now rewrite !app_length.
-  - destruct l; cbn; auto. rewrite !app_length. f_equal. rewrite !map_length. cbn. rewrite !app_length. cbn. lia.
-  - destruct l0; cbn; auto. rewrite !app_length. f_equal. rewrite !app_length. cbn. rewrite !map_length. cbn. rewrite !app_length. cbn. lia.
-Qed.
-  
-
-
-
 Definition encode_tapes (sig : Type) (n : nat) (t : tapes sig n) :=
   encode_list (@Encode_tape sig) (vector_to_list t).
 
@@ -120,74 +102,7 @@ Instance Encode_tapes (sig : Type) (n : nat) : codable (sigList (sigTape sig)) (
 
 (* Compute encode_tapes [| niltape nat; midtape [3;2;1] 4 [5;6;7]; leftof 1 [2;3];rightof 3 [2;1] |]. *)
 
-
-Fixpoint split_vector {X : Type} {n : nat} (v : Vector.t X n) (k : nat) : Vector.t X (min k n) * Vector.t X (n-k).
-Proof.
-  destruct k as [ | k']; cbn.
-  - split. apply Vector.nil.
-    eapply Vector.cast. apply v. abstract lia.
-  - destruct v as [ | x n' v']; cbn.
-    + split. apply Vector.nil. apply Vector.nil.
-    + specialize (split_vector X n' v' k') as (rec1&rec2).
-      split. apply Vector.cons. apply x. apply rec1. apply rec2.
-Defined. (* because definition *)
-
-
 Lemma vector_cast_refl (X : Type) (n1 : nat) (H1 : n1 = n1) (v : Vector.t X n1) :
   Vector.cast v H1 = v.
 Proof. induction v; cbn; f_equal; auto. Qed.
 
-Lemma vector_cast_ext (X : Type) (m n : nat) (H1 H2 : n = m) (v : Vector.t X n) :
-  Vector.cast v H1 = Vector.cast v H2.
-Proof.
-  revert H1 H2. revert m. induction v as [ | x n v IH]; intros.
-  - cbn. destruct m. reflexivity. congruence.
-  - cbn. destruct m. congruence. f_equal. auto.
-Qed.
-
-Lemma vector_cast_2 (X : Type) (n m : nat) (H1 : n = m) (H2 : m = n) (v : Vector.t X n) :
-  Vector.cast (Vector.cast v H1) H2 = v.
-Proof.
-  revert H2 H1. revert m. induction v as [ | x n v IH]; intros.
-  - cbn. destruct m; cbn. reflexivity. congruence.
-  - cbn. destruct m; cbn. congruence. f_equal. auto.
-Qed.
-
-
-Lemma split_vector_correct (X : Type) (n : nat) (v : Vector.t X n) (k : nat) (H : min k n + (n-k) = n) :
-  Vector.cast (Vector.append (fst (split_vector v k)) (snd (split_vector v k))) H = v.
-Proof.
-  revert n v H. induction k as [ | k IH]; intros; cbn.
-  - destruct v; cbn; f_equal. apply vector_cast_2.
-  - revert k H IH. destruct v as [ | x n v]; intros.
-    + cbn. reflexivity.
-    + cbn. specialize (IH _ v (f_equal Init.Nat.pred H)). destruct (split_vector v k) as [rec1 rec2] eqn:E. cbn in *. f_equal. auto.
-Qed.
-
-Lemma split_nat (n k : nat) : min k n + (n-k) = n.
-Proof.
-  revert n. induction k as [ | ? IH]; intros; cbn.
-  - lia.
-  - destruct n; cbn; f_equal; auto.
-Qed.
-  
-
-(* Compute split_vector [| 1; 2; 3; 4 |] 1. *)
-(* Compute let (x,y) := split_vector [| 1; 2; 3; 4 |] 1 in Vector.append x y. *)
-
-
-Lemma sizeOfTape_encodeTape sig' (t : tape sig') :
-| encode_tape t | = let l := sizeOfTape t in if 0 =? l then 1 else 2 + sizeOfTape t.
-Proof.
-  destruct t;cbn - [Nat.eqb].
-  all:repeat (autorewrite with list;cbn [length]).
-  1:easy.
-  2,3:rewrite !Nat.add_succ_r. all:cbn [Nat.eqb]. all:Lia.nia.
-Qed.
-
-
-Lemma sizeOfTape_encodeTape_le sig' (t : tape sig') :
-| encode_tape t | <= 2 + sizeOfTape t.
-Proof.
-  rewrite sizeOfTape_encodeTape. cbn;destruct _;Lia.nia.
-Qed.
